src/ADTNotation.v
@@ -5,5 +5,5 @@ Require Export Fiat.Common.ilist Fiat.Common.BoundedLookup
         Fiat.ADTNotation.BuildComputationalADT.
 
 Open Scope ADT.
-Open Scope ADTParsing.
+Open Scope ADTParsing_scope.
 Open Scope ADTSig.
