src/Parsers/ParserADTSpecification.v
@@ -22,56 +22,56 @@ Section ReferenceImpl.
         Constructor "new" : String.string -> rep,
         (** Initialize, with a given [string] to be parsed or split. *)
 
-        Method "to_string" : rep x unit -> rep x String.string,
+        Method "to_string" : rep -> rep * String.string,
         (** Return the underlying string; hack to get around not having [eq : rep x rep -> bool] *)
 
-        Method "is_char" : rep x Char -> rep x bool,
+        Method "is_char" : rep * Char -> rep * bool,
         (* Return [true] if this string represents a singleton character equal to the given one; otherwise return [false]. *)
 
-        Method "get" : rep x nat -> rep x option Char,
+        Method "get" : rep * nat -> rep * (option Char),
         (* Returns [Some ch] if the [n]th character of this string is some [ch], and returns [None] otherwise. *)
 
-        Method "length" : rep x unit -> rep x nat,
+        Method "length" : rep -> rep * nat,
         (** Return the length of this string. *)
 
-        Method "take" : rep x nat -> rep x unit,
+        Method "take" : rep * (nat : Type) -> rep,
         (** Return the first [n] characters, for the given [n : nat]. *)
 
-        Method "drop" : rep x nat -> rep x unit,
+        Method "drop" : rep * (nat : Type) -> rep,
         (** Return everything but the first [n] characters, for the given [n : nat]. *)
 
-        Method "splits" : rep x item Char * production Char -> rep x list nat
+        Method "splits" : rep * (item Char) * (production Char) -> rep * (list nat)
         (** Return a list of locations to split this string at for this production rule. *)
       }.
   End GenericSig.
 
   Context (G : grammar Ascii.ascii).
-
+  Local Open Scope ADTParsing_scope.
   (** Reference implementation of a [String] that can be split *)
   Definition string_spec : ADT (string_rep Ascii.ascii) := ADTRep String.string {
-    Def Constructor "new"(s : String) : rep :=
+    Def Constructor1 "new"(s : String) : rep :=
       ret s,
 
-    Def Method "to_string"(s : rep, x : unit) : String.string :=
+    Def Method0 "to_string" (s : rep) : rep * String.string :=
       ret (s, s),
 
-    Def Method "is_char"(s : rep, x : Ascii.ascii) : bool  :=
+    Def Method1 "is_char"(s : rep) (x : Ascii.ascii) : rep * bool  :=
       ret (s, string_beq s (String.String x "")),
 
-    Def Method "get"(s : rep, n : nat) : option Ascii.ascii  :=
+    Def Method1 "get"(s : rep) (n : nat) : rep * (option Ascii.ascii)  :=
       ret (s, get n s),
 
-    Def Method "length"(s : rep, x : unit) : nat :=
+    Def Method0 "length"(s : rep) : rep * nat :=
       ret (s, String.length s),
 
-    Def Method "take"(s : rep, n : nat) : unit :=
-      ret (take n s, tt),
+    Def Method1 "take"(s : rep) (n : nat) : rep :=
+      ret (take n s),
 
-    Def Method "drop"(s : rep, n : nat) : unit :=
-      ret (drop n s, tt),
+    Def Method1 "drop"(s : rep) (n : nat) : rep :=
+      ret (drop n s),
 
-    Def Method "splits"(s : rep, p : item Ascii.ascii * production Ascii.ascii) : list nat :=
-      ls <- { ls : list nat | split_list_is_complete G s (fst p) (snd p) ls };
+    Def Method2 "splits"(s : rep) (i : item Ascii.ascii) (p : production Ascii.ascii) : rep * list nat :=
+      ls <- { ls : list nat | split_list_is_complete G s i p ls };
       ret (s, ls)
   }.
 End ReferenceImpl.
